Option to use LV in `solve_by_wp`
`O_LV`

dist/experiment.c
@@ -12,6 +12,12 @@ void Experiment_Steel_Test_Extract_test3(uint32_t *r0, uint32_t *r1)
   r1[0U] = x + (uint32_t)1U;
 }
 
+void Experiment_Steel_Test_Extract_test3_LV(uint32_t *r0, uint32_t *r1)
+{
+  uint32_t x = r0[0U];
+  r1[0U] = x + (uint32_t)1U;
+}
+
 uint32_t Experiment_Steel_Test_Extract_test_ghost(uint32_t *r)
 {
   return r[0U];
