dist/experiment.h
@@ -12,6 +12,8 @@
 #include "krml/internal/target.h"
 void Experiment_Steel_Test_Extract_test3(uint32_t *r0, uint32_t *r1);
 
+void Experiment_Steel_Test_Extract_test3_LV(uint32_t *r0, uint32_t *r1);
+
 uint32_t Experiment_Steel_Test_Extract_test_ghost(uint32_t *r);
 
 
