experiment/Experiment.Steel.fst
@@ -7,9 +7,9 @@ module SF2Fun = Experiment.Steel.Repr.SF_to_Fun
 #set-options "--ide_id_info_off --ifuel 0"
 
 (**) #push-options "--ifuel 0"
-(**) private let __begin_prog_M_to_Fun = ()
+(**) private let __begin_prog_to_Fun = ()
 (**) #pop-options
-(**) private let __end_prog_M_to_Fun = ()
+(**) private let __end_prog_to_Fun = ()
 
 
 #push-options "--z3rlimit 20"
@@ -95,6 +95,36 @@ let prog_M_to_Fun_equiv
         Fun.tree_ens t_Fun' xsl1;
       }
     end
+
+#pop-options
+
+#push-options "--ifuel 0 --fuel 0"
+let prog_LV_to_Fun_equiv_M
+      (#ek : SH.effect_kind) (#a : Type) (t : M.repr ek a)
+      (#pre : M.pre_t) (#post : M.post_t a)
+      (lc : LV.top_lin_cond t.repr_tree pre post {LV.lcsub_at_leaves lc})
+      (sl0 : Vpl.sl_f pre)
+  : Lemma (prog_M_equiv_Fun t.repr_tree (LV2M.repr_M_of_LV_top lc) sl0 (prog_LV_to_Fun t lc sl0))
+  =
+    let tr    = t.repr_tree                in
+    let mc    = LV2M.repr_M_of_LV_top lc   in
+    let t_SF  = LV2SF.repr_SF_of_LV lc sl0 in
+    let t_Fun = prog_LV_to_Fun t lc sl0    in
+
+    LV2M.repr_M_of_LV_top_sound lc;
+    LV2SF.repr_SF_of_LV_sound lc sl0;
+    SF2Fun.repr_Fun_of_SF_req t_SF;
+
+    let lem_req () : Lemma (M.tree_req t.repr_tree mc sl0 <==> Fun.tree_req t_Fun) = () in
+    let lem_ens (x : a) (sl1 : Vpl.sl_f (post x))
+      : Lemma (M.tree_ens tr mc sl0 x sl1 <==> Fun.tree_ens t_Fun ({val_v = x; sel_v = sl1}))
+      = SF2Fun.repr_Fun_of_SF_ens t_SF x sl1
+    in
+    assert (prog_M_equiv_Fun t.repr_tree (LV2M.repr_M_of_LV_top lc) sl0 (prog_LV_to_Fun t lc sl0))
+      by (norm [delta_only [`%prog_M_equiv_Fun]];
+          split ();
+            apply_lemma (``@lem_req);
+            let _ = mintros () in apply_lemma (``@lem_ens))
 #pop-options
 
 
