experiment/Experiment.Steel.Repr.LV_to_SF.fsti
@@ -10,34 +10,30 @@ open Experiment.Steel.Repr.LV
 
 #set-options "--fuel 1 --ifuel 1"
 
-let post_SF_of_LV (#a : Type u#a) (prd : prd_t a) (x : a)
-  : Fl.ty_list
-  = vprop_list_sels_t (prd x)
-
 [@@ strict_on_arguments [5]] (* strict on [lc] *)
 let rec repr_SF_of_LV
       (#env : vprop_list) (#a : Type u#a) (#t : M.prog_tree a)
       (#csm : csm_t env) (#prd : prd_t a)
       (lc : lin_cond env t csm prd)
       (sl0 : sl_f env)
-  : Tot (SF.prog_tree a (post_SF_of_LV prd)) (decreases lc)
+  : Tot (SF.prog_tree a (M.post_sl_t prd)) (decreases lc)
   = match lc with
   | LCspec env #a #pre #post #req #ens csm_f ->
       let sl0' = eij_sl (L.index csm_f) sl0 in
-      SF.Tspec a (post_SF_of_LV post) (req sl0') (ens sl0')
+      SF.Tspec a (M.post_sl_t post) (req sl0') (ens sl0')
   | LCret  env #a #x prd csm_f ->
-      SF.Tret a x (post_SF_of_LV prd) (Fl.dlist_of_f (eij_sl (L.index csm_f) sl0))
+      SF.Tret a x (M.post_sl_t prd) (Fl.dlist_of_f (eij_sl (L.index csm_f) sl0))
   | LCbind env #a #b f_csm f_prd cf g_csm g_prd cg ->
-      SF.Tbind a b (post_SF_of_LV f_prd) (post_SF_of_LV g_prd)
+      SF.Tbind a b (M.post_sl_t f_prd) (M.post_sl_t g_prd)
                (repr_SF_of_LV cf sl0)
                (fun (x : a) (sl1 : sl_f (f_prd x)) ->
                   repr_SF_of_LV (cg x) (res_sel sl0 f_csm sl1))
   | LCsub  env csm0 prd0 cf csm1 prd1 prd_f ->
-      SF.Tbind a a (post_SF_of_LV prd0) (post_SF_of_LV prd1)
+      SF.Tbind a a (M.post_sl_t prd0) (M.post_sl_t prd1)
                (repr_SF_of_LV cf sl0)
                (fun (x : a) (sl1 : sl_f (prd0 x)) ->
                   let sl1' : sl_f (prd1 x) = sub_prd_sl #env sl0 csm0 sl1 csm1 (prd_f x) in
-                  SF.Tret a x (post_SF_of_LV prd1) (Fl.dlist_of_f sl1'))
+                  SF.Tret a x (M.post_sl_t prd1) (Fl.dlist_of_f sl1'))
 
 
 (*** Soundness *)
@@ -47,7 +43,7 @@ let sound_SF_of_LV
       (#csm : csm_t env) (#prd : prd_t a)
       (lc : lin_cond env t csm prd)
       (sl0 : sl_f env)
-      (sf : SF.prog_tree a (post_SF_of_LV prd))
+      (sf : SF.prog_tree a (M.post_sl_t prd))
   : prop
   =
     (tree_req lc sl0 <==> SF.tree_req sf) /\
